src/examples/rwlock.v
@@ -1,0 +1,237 @@
+From iris.base_logic.lib Require Import invariants.
+From BurrowLang Require Import lang simp adequacy primitive_laws.
+From Tpcms Require Import rwlock.
+Require Import Burrow.tpcms.
+Require Import Burrow.ra.
+Require Import Burrow.rollup.
+
+From iris.base_logic Require Export base_logic.
+From iris.program_logic Require Export weakestpre.
+From iris.proofmode Require Import tactics.
+From iris.program_logic Require Import ectx_lifting.
+From BurrowLang Require Import notation tactics class_instances.
+From BurrowLang Require Import heap_ra.
+From BurrowLang Require Import lang.
+From iris Require Import options.
+
+Definition loop_until e : lang.expr :=
+    (rec: "loop" "c" :=
+      if: e then #()
+      else "loop" "c") #0.
+
+Definition new_rwlock : lang.expr :=
+  Pair (ref #0) (ref #0).
+
+Definition acquire_exc : lang.expr :=
+  λ: "rw" ,
+    loop_until (CAS (Fst "rw") #0 #1) ;;
+    loop_until (op_eq (!(Snd "rw")) #0).
+
+Definition release_exc : lang.expr :=
+  λ: "rw" ,
+    Fst "rw" <- #0.
+    
+Definition acquire_shared : lang.expr :=
+  λ: "rw" ,
+    loop_until (
+      FAA (Snd "rw") #1 ;;
+      if: op_eq (!(Fst "rw")) #0 then
+        #1
+      else (
+        FAA (Snd "rw") (#(-1)) ;;
+        #0
+      )
+    ).
+    
+Definition release_shared : lang.expr :=
+  λ: "rw" ,
+    FAA (Snd "rw") (#(-1)).
+    
+
+Section RwlockProof.
+
+Context {𝜇: BurrowCtx}.
+
+Context {M} `{!EqDecision M} `{!TPCM M}.
+Context `{!HasTPCM 𝜇 M}.
+Context `{!HasTPCM 𝜇 (RwLock M)}.
+Context `{!HasRef 𝜇 (rwlock_ref M)}.
+
+Context `{!simpGS 𝜇 Σ}.
+
+Definition NS := nroot .@ "rwlock".
+
+Definition rwlock_inv 𝛼 𝛾 (contents_inv: M -> Prop) l1 l2 : iProp Σ :=
+  (∃ exc rc x ,
+    L (rwloc 𝛼 𝛾) (Central exc rc x)
+    ∗ ⌜ contents_inv x ⌝
+    ∗ (l1 ↦ (LitV (LitInt (match exc with false => 0 | true => 1 end))))
+    ∗ (l2 ↦ (LitV (LitInt rc)))
+  ).
+  
+Global Instance rwlock_inv_timeless 𝛼 𝛾 contents_inv l1 l2 : Timeless (rwlock_inv 𝛼 𝛾 contents_inv l1 l2). Admitted.
+
+Definition is_rwlock rwlock 𝛼 𝛾 (contents_inv: M -> Prop) : iProp Σ :=
+  match rwlock with
+    | PairV (LitV (LitInt l1)) (LitV (LitInt l2)) =>
+        inv NS (rwlock_inv 𝛼 𝛾 contents_inv l1 l2)
+    | _ => False
+  end.
+  
+Global Instance is_rwlock_persistent rwlock 𝛼 𝛾 contents_inv : Persistent (is_rwlock rwlock 𝛼 𝛾 contents_inv). Admitted.
+
+Lemma hoare_new_rwlock (𝛾: BurrowLoc 𝜇) (x: M) (contents_inv: M -> Prop)
+    (sat_inv: contents_inv x) :
+  {{{ L 𝛾 x }}} new_rwlock
+  {{{ rwlock 𝛼 , RET rwlock ; is_rwlock rwlock 𝛼 𝛾 contents_inv }}}.
+Proof.
+  iIntros (Phi) "H Q".
+  unfold new_rwlock.
+  wp_alloc b_ref as "rb".
+  wp_alloc a_ref as "ra".
+  iMod (rw_new _ _ with "H") as (𝛼) "H".
+  iAssert (rwlock_inv 𝛼 𝛾 contents_inv a_ref b_ref) with "[rb ra H]" as "ri".
+  - unfold rwlock_inv. iExists false. iExists 0. iExists x. iFrame. iPureIntro. trivial.
+  - iMod (inv_alloc NS _ _ with "ri") as "i".
+    wp_pures.
+    iApply "Q".
+    iModIntro.
+    iFrame.
+Qed.
+
+Lemma loop_w_invariant e (P Q R : iProp Σ)
+  (hr: {{{ Q }}} e {{{ n, RET #n ; (⌜n=0⌝ -∗ Q) ∗ (⌜n=1⌝ -∗ R) ∗ (⌜n=0 \/ n=1⌝) }}})
+  (eokay: (∀ X Y , subst "c" Y (subst "loop" X e) = e))
+  (entry: P ⊢ Q)
+  : {{{ P }}} loop_until e {{{ RET #(); R }}}.
+Proof.
+  iIntros (phi) "p x".
+  iDestruct (entry with "p") as "q".
+  unfold loop_until.
+  wp_pures.
+  iLöb as "IH".
+  rewrite eokay.
+  wp_apply (hr with "q").
+  iIntros "%n [w [v u]]".
+  have h : Decision (n=0) by solve_decision. destruct h.
+  - subst n.
+    wp_pures. rewrite eokay. 
+    iApply ("IH" with "x").
+    iApply "w".
+    iPureIntro. trivial.
+  - have h : Decision (n=1) by solve_decision. destruct h.
+     + subst n. wp_pures. iModIntro. iApply "x". iApply "v". iPureIntro. trivial.
+     + iDestruct "u" as "%u". lia.
+Qed.
+
+From BurrowLang Require Import class_instances.
+
+(*
+From iris.algebra Require Import excl.
+
+Definition join : val :=
+  rec: "join" "c" :=
+    let: "r" := !"c" in
+    if: Fst "r" then Snd "r"
+    else "join" "c".
+    
+Definition NONE: expr := (#false, #()).
+Definition NONEV: val := (#false, #()).
+
+Definition SOME: expr := λ: "v", (#true, "v").
+Definition SOMEV (v:val): val := (#true, v).
+
+Class spawnG Σ := SpawnG { spawn_tokG :> inG Σ (exclR unitO) }.
+Definition spawnΣ : gFunctors := #[GFunctor (exclR unitO)].
+
+Global Instance subG_spawnΣ : subG spawnΣ Σ → spawnG Σ.
+Proof. solve_inG. Qed.
+
+Context `{!simpGS 𝜇 Σ, !spawnG Σ} (N : namespace).
+    
+Definition spawn_inv (γ : gname) (l : loc) (Ψ : val → iProp Σ) : iProp Σ :=
+  ∃ lv, l ↦ lv ∗ (⌜lv = NONEV⌝ ∨
+                  ∃ w, ⌜lv = SOMEV w⌝ ∗ (Ψ w ∨ own γ (Excl ()))).
+    
+Definition join_handle (l : loc) (Ψ : val → iProp Σ) : iProp Σ :=
+  ∃ γ, own γ (Excl ()) ∗ inv N (spawn_inv γ l Ψ).
+  *)
+
+(*
+Lemma join_spec (Ψ : val → iProp Σ) l :
+  {{{ join_handle l Ψ }}} join #l {{{ v, RET v; Ψ v }}}.
+Proof.
+  iIntros (Φ) "H HΦ". iDestruct "H" as (γ) "[Hγ #?]".
+  iLöb as "IH". unfold join. wp_rec. wp_bind (! _)%E. iInv N as (v) "[Hl Hinv]".
+  wp_load. iDestruct "Hinv" as "[%|Hinv]"; subst.
+  - iModIntro. iSplitL "Hl"; [iNext; iExists _; iFrame; eauto|].
+    wp_pures. 
+    wp_apply ("IH" with "Hγ [HΦ]"). auto.
+  - iDestruct "Hinv" as (v' ->) "[HΨ|Hγ']".
+    + iModIntro. iSplitL "Hl Hγ"; [iNext; iExists _; iFrame; eauto|].
+      wp_pures. by iApply "HΦ".
+    + iDestruct (own_valid_2 with "Hγ Hγ'") as %[].
+Qed.
+End proof.
+*)
+
+
+Lemma acq1 (rwlock: lang.val) 𝛼 𝛾 contents_inv :
+      {{{ is_rwlock rwlock 𝛼 𝛾 contents_inv }}}
+      loop_until (CAS (Fst rwlock) #0 #1)
+      {{{ RET #(); L (rwloc 𝛼 𝛾) ExcPending }}}.
+Proof.
+  iIntros (phi) "#isr p".
+  wp_apply (loop_w_invariant _ (is_rwlock rwlock 𝛼 𝛾 contents_inv)%I (is_rwlock rwlock 𝛼 𝛾 contents_inv)%I (L (rwloc 𝛼 𝛾) ExcPending ∗ is_rwlock rwlock 𝛼 𝛾 contents_inv)%I).
+  - iIntros (phi2) "#t p".
+      unfold is_rwlock. destruct rwlock; try (destruct rwlock1, rwlock2).
+        + iExFalso. iFrame "#".
+        + iExFalso. iFrame "#".
+        + destruct l, l0.
+          * wp_pures. iInv "t" as (exc rc) ">I".
+              iDestruct "I" as (x) "I".
+              iDestruct "I" as "[L [c [a b]]]".
+            unfold rwlock_inv.
+            wp_apply (wp_cas with "a").
+            destruct exc.
+              -- case_decide.
+                ++ exfalso. inversion H.
+                ++ iIntros "n1". iModIntro. iSplitR "p".
+                  ** iModIntro. iExists true, rc, x. iFrame.
+                  ** simpl. iApply ("p" $! 0). iSplit.
+                    --- iIntros. iFrame "#".
+                    --- iSplit.
+                      +++ iIntros "%". inversion H0.
+                      +++ iPureIntro. lia.
+              -- case_decide.
+                ++ iIntros "n1".
+                  iMod (rw_exc_begin with "L") as "[L pend]". iModIntro. iSplitR "p pend".
+                   ** iModIntro. iExists true, rc, x. iFrame.
+                   ** simpl. iApply ("p" $! 1). iSplit.
+                    --- iIntros "%". inversion H0.
+                    --- iSplitL "pend".
+                      +++ iIntros. iFrame "#". iFrame.
+                      +++ iPureIntro. lia.
+                ++ contradiction.
+          * iExFalso. iFrame "#".
+          * iExFalso. iFrame "#".
+          * iExFalso. iFrame "#".
+        + iExFalso. destruct l.
+          * iFrame "#".
+          * iFrame "#".
+        + iExFalso. destruct l.
+          * iFrame "#".
+          * iFrame "#".
+        + iExFalso. iFrame "#".
+        + iExFalso. iFrame "#".
+        + iExFalso. iFrame "#".
+        + iExFalso. iFrame "#".
+        + iExFalso. iFrame "#".
+        + iExFalso. iFrame "#".
+    - intros. trivial.
+    - iIntros. iFrame "#".
+    - iFrame "#".
+    - iIntros "[x y]". iApply "p". iFrame.
+Qed.
+
+End rwlockProof.
